%-------------------------------------------------------------------------------
%   PACKAGES AND OTHER DOCUMENT CONFIGURATIONS
%-------------------------------------------------------------------------------
\documentclass[paper=a4, fontsize=11pt]{scrartcl} % A4 paper and 11pt font size
\usepackage{fancyhdr} % Required for custom headers
\usepackage{lastpage} % Required to determine the last page for the footer
\usepackage{extramarks} % Required for headers and footers
\usepackage[usenames,dvipsnames]{color} % Required for custom colors
\usepackage{graphicx} % Required to insert images
\usepackage{listings} % Required for insertion of code
\usepackage{courier} % Required for the courier font
\usepackage[T1]{fontenc} % Use 8-bit encoding that has 256 glyphs
\usepackage[english]{babel} % English language/hyphenation
\usepackage{amsmath,amsfonts,amsthm} % Math packages

\usepackage{sectsty} % Allows customizing section commands
\allsectionsfont{\centering \normalfont\scshape} % Make all sections centered, 
                                                 % the default font and small 
                                                 % caps

\pagestyle{fancyplain} % Makes all pages in the document conform to the custom
                       % headers and footers
\fancyhead{} % No page header - if you want one, create it in the same way as 
             % the footers below
\fancyfoot[L]{} % Empty left footer
\fancyfoot[C]{} % Empty center footer
\fancyfoot[R]{\thepage} % Page numbering for right footer
\renewcommand{\headrulewidth}{0pt} % Remove header underlines
\renewcommand{\footrulewidth}{0pt} % Remove footer underlines
\setlength{\headheight}{13.6pt} % Customize the height of the header

\numberwithin{equation}{section} % Number equations within sections (i.e. 1.1, 
                                 % 1.2, 2.1, 2.2 instead of 1, 2, 3, 4)
\numberwithin{figure}{section} % Number figures within sections (i.e. 1.1, 1.2,
                               % 2.1, 2.2 instead of 1, 2, 3, 4)
\numberwithin{table}{section} % Number tables within sections (i.e. 1.1, 1.2, 
                              % 2.1, 2.2 instead of 1, 2, 3, 4)

\setlength\parindent{0pt} % Removes all indentation from paragraphs - comment 
                          % this line for an assignment with lots of text

%-------------------------------------------------------------------------------
%   TITLE SECTION
%-------------------------------------------------------------------------------

\newcommand{\horrule}[1]{\rule{\linewidth}{#1}} % horizontal cmd, arg = height
\newcommand{\name}{Colin Bradford} % student name
\newcommand{\hwnum}{3} % homework number
\newcommand{\classnum}{CS 325} % class num with abreviation
\newcommand{\classname}{Analysis of Algorithms} % name of class
\newcommand{\hwtitle}{\classnum: Homework \hwnum}
\newtheorem{theorem}{Theorem}[section]

\title{ 
    \normalfont \normalsize 
    \textsc{Oregon State University} \\ [25pt]
    \horrule{0.5pt} \\[0.4cm] % Thin top horizontal rule
    \huge \hwtitle \\ % The assignment title
    \horrule{2pt} \\[0.5cm] % Thick bottom horizontal rule
}

\author{\name} % Your name

\date{\normalsize\today} % Today's date or a custom date

%-------------------------------------------------------------------------------
%   DOCUMENT
%-------------------------------------------------------------------------------
\begin{document}

\maketitle % Print the title

\begin{enumerate}
    %   PROBLEM 1
    \item \hfill \\
    \begin{enumerate}
        \item $T(n) = \Theta(n^2)$
        \begin{proof}
            Given $T(n) = T(n - 2) + n$ \\
            Let $k$ be the number of iterations for any given $n$ \\
            Since the size $n$ is reduce by 2 each iteration, then after some 
            $k$ iterations $n = 1$ which will be the $T(1)$ case. Thus we know
            that $n - 2k = 1$. Rewritten the equation looks like 
            \begin{equation}
                k = \frac{ n - 1 }{ 2 }
            \end{equation}
            Next it will be shown that $T(n) \approx n^2$ \\
            Given the arithmetic series
            \begin{equation}
                \sum\limits_{i=1}^k i = \frac{(k)(k + 1)}{2}
            \end{equation}
            then using the iterative method we can show
            \begin{align*}
                T(n) &= T(n - 2) + n \\
                T(n - 2) &= T(n - 4) + n - 2 \\
                \ldots &= n +(n - 2 +(n - 4 + (\ldots))) \\
                &= (n + n + \ldots + n) + (- 2 - 4 - \ldots - 2k) \\
                &= kn + (-2)\sum\limits_{i=1}^k i \\
                &= kn - 2\left(\frac{(k)(k + 1)}{2}\right) \tag{eq. 0.2} \\
                &= kn - (k)(k + 1) \\
                &= \left(\frac{ n - 1 }{ 2 }\right)\left(n\right) - 
                \left(\frac{ n - 1 }{ 2 }\right)\left(\frac{ n - 1 }{ 2 } + 
                \frac{ 2 }{ 2 }\right)  \tag{eq. 0.1}\\
                &= \frac{ n^2 - n }{ 2 } - 
                \left(\frac{ n - 1 }{ 2 }\right)\left(
                \frac{ n + 1 }{ 2 }\right) \\
                &= \frac{ n^2 - n }{ 2 } - \frac{ n^2 - 1 }{ 4 } \\
                &= \frac{ 2n^2 - 2n }{ 4 } - \frac{ n^2 - 1 }{ 4 } \\
                T(n) &= \frac{ n^2 - 2n + 1 }{ 4 } \\
            \end{align*}
            Thus we can see that $T(n)$ must be $\Theta(n^2)$.
        \end{proof}

    \item $T(n) = \Theta(n)$
    \begin{proof}
        Given $T(n) = T(n - 1) + 3$ \\
        Let $k$ be the number of iterations for any given $n$ \\
        Since the size $n$ is reduce by 1 each iteration, then after some 
        $k$ iterations $n = 1$ which will be the $T(1)$ case. Thus we know
        that $n - k = 0$ assuming we don't care about the $T(1)$ case. 
        Rewritten the equation looks like 
        \begin{equation}
            k = n
        \end{equation}
        Using the iterative method we can show
        \begin{align*}
            T(n) = T(n - 1) + 3 \\
            T(n - 1) = T(n - 2) + 3 \\
            \ldots = 3 + (3 + (3 + (\ldots))) \\
            T(n) = 3k \\
            T(n) = 3n \tag{eq 0.3} \\
        \end{align*}
        Thus we know that $T(n)$ must be $\Theta(n)$.
    \end{proof}

    \item $T(n) = \Theta(n)$
    \begin{proof}
        Given $T(n) = 2T(\frac{ n }{ 4 }) + n$ \\
        \begin{theorem}[Master's theorem]
            Let $a \in \mathbb{Z}$ and $a \geq 1$, and $b \in \mathbb{R}$ and 
            $b \geq 1$. Let $c \in \mathbb{R}$ and $c > 0$, and 
            $d \in \mathbb{R}$ and $d \geq 0$. Given a recurrence of the form
        \[
            T(n) = 
            \begin{cases}
                aT(n/b) n^c, & \text{if $n > 1$}.\\
                d, & \text{if $n = 1$}.
            \end{cases} 
        \]
        then for n a power of b,
        \begin{enumerate}
            \item if $\log_b{a} < c$, $T(n) = \Theta\left(n^c\right)$
            \item if $\log_b{a} = c$, $T(n) = \Theta\left(n^c\log{n}\right)$
            \item if $\log_b{a} > c$, $T(n) = \Theta\left(n^{ \log_b{a} }\right)$
        \end{enumerate}
        \end{theorem}
        Using the Master's theorem, let $a = 2$, $b = 4$, and $c = 1$ \\
        Assume, $\log_b{a} < c$ and as a result $T(n) = \Theta\left(n^c\right)$
        \begin{align*}
            \log_4{2} &< 1 \\
            4^{\log_4{2}} &< 4^1 \\
            2 &< 4
        \end{align*}
        Thus we know that $T(n) = \Theta\left(n^1\right) = \Theta(n)$.
    \end{proof}

    \item $T(n) = \Theta(n^{\frac{ 5 }{ 2 }})$
    \begin{proof}
        Given $T(n) = 4T(\frac{ n }{ 2 }) + n^2\sqrt{n}$ \\
        We can rewrite this equation to be
        \[ 4T(\frac{ n }{ 2 }) + n^{5/2} \]
        Using the Master's theorem, $a = 4$, $b = 2$, and $c = \frac{5}{2}$ \\
        Assume, $\log_b{a} < c$ and as a result $T(n) = \Theta\left(n^c\right)$
        \begin{align*}
            \log_2{4} & < \frac{5}{2} \\
            2 & < \frac{5}{2} \\
            \frac{4}{2} & < \frac{5}{2} \\
            4 & < 5
        \end{align*}
        Thus we know that $T(n) = \Theta\left(n^{5/2}\right)$.
    \end{proof}
    \end{enumerate}

    %   PROBLEM 2
    \item \hfill \\

    %   PROBLEM 3
    \item \hfill \\

    %   PROBLEM 4
    \item \hfill \\
    \begin{lstlisting}[language=Python]
    Ternary-Sort(sTerm, list, low, high):
        n = high - low
        lowMid = n / 3 + low
        highMid = (2 * n) / 3 + low

        if (sTerm == list[lowMid]):
            return lowMid
        else if(sTerm == list[highMid]):
            return highMid
        else if (n == 0):
            return -1
        else if (sTerm < list[lowMid]):
            return Ternary-Sort(sTerm, list, low, lowMid)
        else if (sTerm < list[highMid]):
            return Ternary-Sort(sTerm, list, lowMid, highMid)
        else
            return Ternary-Sort(sTerm, list, highMid, high)
    \end{lstlisting}
    %   PROBLEM 5
    \item \hfill \\
\end{enumerate}
\end{document}
%-------------------------------------------------------------------------------


